src/tls/DHGroup.fst
@@ -100,6 +100,9 @@ val dh_initiator: #g:group -> keyshare g -> share g -> ST (secret g)
 let dh_initiator #g x gy =
   dh_agreement x gy
 
+
+/// Parsing and formatting (TODO: check against RFC)
+/// 
 val serialize: #g:group -> share g -> Tot (b:bytes{length b < 196612})
 let serialize #g dh_Y =
   let dhp = params_of_group g in
